helping/Header.v
@@ -1,8 +1,7 @@
 Require Import CRIS.
 
 Module Helping. Section Helping.
-
-  Context `{Σ: GRA}.
+  Context `{Σ : GRA}.
   Context (mn : string).
 
   Definition run  := mn +:+ ".run".
@@ -14,5 +13,4 @@ Module Helping. Section Helping.
     translate (case_ (bif:=sum1) subevent subevent) itr.
 
   Definition exports := [run; help].
-
 End Helping. End Helping.
